===================================================                   Isabelle + HOLA ===================================================

docs/src/internal/formal/VM_Register.thy
@@ -1,5 +1,5 @@
 theory VM_Register
-  imports Physics_Formal.VM_Words
+  imports VM_Words VM_DataStack_Words
 begin
 
 section \<open>Dictionary registration model\<close>
@@ -10,23 +10,36 @@ text \<open>
   semantic function (state → state).
 \<close>
 
-type_synonym ('dict,'val,'io) word_dict =
-  "(string \<times> (('dict,'val stack,'io) vm_core_state \<Rightarrow> ('dict,'val stack,'io) vm_core_state)) list"
+type_synonym ('dict,'val,'io,'phys) word_dict =
+  "(string \<times> (('dict,'val stack,'io,'phys) vm_core_state \<Rightarrow> ('dict,'val stack,'io,'phys) vm_core_state)) list"
 
-fun lookup_word :: "string \<Rightarrow> ('d,'v,'i) word_dict \<Rightarrow> (('d,'v stack,'i) vm_core_state \<Rightarrow> ('d,'v stack,'i) vm_core_state) option" where
+fun lookup_word :: "string \<Rightarrow> ('d,'v,'i,'p) word_dict \<Rightarrow> (('d,'v stack,'i,'p) vm_core_state \<Rightarrow> ('d,'v stack,'i,'p) vm_core_state) option" where
   "lookup_word _ [] = None" |
   "lookup_word name ((n,f)#rest) = (if name = n then Some f else lookup_word name rest)"
 
-definition register_word :: "string \<Rightarrow> (('d,'v stack,'i) vm_core_state \<Rightarrow> ('d,'v stack,'i) vm_core_state) \<Rightarrow> ('d,'v,'i) word_dict \<Rightarrow> ('d,'v,'i) word_dict" where
+definition register_word :: "string \<Rightarrow> (('d,'v stack,'i,'p) vm_core_state \<Rightarrow> ('d,'v stack,'i,'p) vm_core_state) \<Rightarrow> ('d,'v,'i,'p) word_dict \<Rightarrow> ('d,'v,'i,'p) word_dict" where
   "register_word name f dict = (name, f) # dict"
 
 context vm_stack_runtime begin
 
-definition register_return_stack_words :: "('dict,'val,'io) word_dict \<Rightarrow> ('dict,'val,'io) word_dict" where
+definition register_return_stack_words :: "('dict,'val,'io,'phys) word_dict \<Rightarrow> ('dict,'val,'io,'phys) word_dict" where
   "register_return_stack_words dict =
       register_word \"R@\" word_peek_return (
       register_word \"R>\" word_from_return (
       register_word \">R\" word_to_return dict))"
+
+definition register_data_stack_words :: "('dict,'val,'io,'phys) word_dict \<Rightarrow> ('dict,'val,'io,'phys) word_dict" where
+  "register_data_stack_words dict =
+      register_word \"ROLL\" word_roll (
+      register_word \"PICK\" word_pick (
+      register_word \"DEPTH\" word_depth (
+      register_word \"-ROT\" word_minus_rot (
+      register_word \"ROT\" word_rot (
+      register_word \"OVER\" word_over (
+      register_word \"SWAP\" word_swap (
+      register_word \"?DUP\" word_qdup (
+      register_word \"DUP\" word_dup (
+      register_word \"DROP\" word_drop dict)))))))))"
 
 lemma lookup_register_word_same:
   "lookup_word name (register_word name f dict) = Some f"
@@ -56,6 +69,51 @@ lemma register_return_stack_words_preserve_other:
   assumes name \notin set [\">R\", \"R>\", \"R@\"]
   shows "lookup_word name (register_return_stack_words dict) = lookup_word name dict"
   using assms unfolding register_return_stack_words_def register_word_def by simp
+
+lemma register_data_stack_words_drop:
+  "lookup_word \"DROP\" (register_data_stack_words dict) = Some word_drop"
+  unfolding register_data_stack_words_def by (simp add: register_word_def)
+
+lemma register_data_stack_words_dup:
+  "lookup_word \"DUP\" (register_data_stack_words dict) = Some word_dup"
+  unfolding register_data_stack_words_def by (simp add: register_word_def)
+
+lemma register_data_stack_words_qdup:
+  "lookup_word \"?DUP\" (register_data_stack_words dict) = Some word_qdup"
+  unfolding register_data_stack_words_def by (simp add: register_word_def)
+
+lemma register_data_stack_words_swap:
+  "lookup_word \"SWAP\" (register_data_stack_words dict) = Some word_swap"
+  unfolding register_data_stack_words_def by (simp add: register_word_def)
+
+lemma register_data_stack_words_over:
+  "lookup_word \"OVER\" (register_data_stack_words dict) = Some word_over"
+  unfolding register_data_stack_words_def by (simp add: register_word_def)
+
+lemma register_data_stack_words_rot:
+  "lookup_word \"ROT\" (register_data_stack_words dict) = Some word_rot"
+  unfolding register_data_stack_words_def by (simp add: register_word_def)
+
+lemma register_data_stack_words_minus_rot:
+  "lookup_word \"-ROT\" (register_data_stack_words dict) = Some word_minus_rot"
+  unfolding register_data_stack_words_def by (simp add: register_word_def)
+
+lemma register_data_stack_words_depth:
+  "lookup_word \"DEPTH\" (register_data_stack_words dict) = Some word_depth"
+  unfolding register_data_stack_words_def by (simp add: register_word_def)
+
+lemma register_data_stack_words_pick:
+  "lookup_word \"PICK\" (register_data_stack_words dict) = Some word_pick"
+  unfolding register_data_stack_words_def by (simp add: register_word_def)
+
+lemma register_data_stack_words_roll:
+  "lookup_word \"ROLL\" (register_data_stack_words dict) = Some word_roll"
+  unfolding register_data_stack_words_def by (simp add: register_word_def)
+
+lemma register_data_stack_words_preserve_other:
+  assumes name \notin set [\"DROP\", \"DUP\", \"?DUP\", \"SWAP\", \"OVER\", \"ROT\", \"-ROT\", \"DEPTH\", \"PICK\", \"ROLL\"]
+  shows "lookup_word name (register_data_stack_words dict) = lookup_word name dict"
+  using assms unfolding register_data_stack_words_def register_word_def by simp
 
 end
 
